### Convolution Systems with Complex Exponential Inputs




### Properties of Convolution
Given
$$(f* g)(t) = \int^{\infty}_{-\infty}f(\tau)g(\tau)d \tau$$
Convolution Integral is 


Commutative 








Example
<to be insert>


Assocaitive



Linear

Time Invariant

### Graphical Interpretation
An increment in input $x(\tau)\delta_{\tau}(t) d\tau$ produces an impulse response $x(\tau)h_{\tau}(t)d\tau$. The output is the integral of all the reponses

$$y(t) = \int^{\infty}_{-\infty}x(\tau)h_{\tau}(t)d \tau$$

Another persepective to look at the integral
- $h_{\tau}(t) = h(t-\tau)$ is the impulse reponse delayed to time $\tau$
- h_{t}(\tau) = h(t-\tau)$ would be a function of $\tau$ and delayed to time t, making the signal flipped

To find $y(t)$
- flip impulse response $$h(\tau)$$ backwards in time (yields $$h(-\tau)$$)
- drag to the right over $$t$$ (yields $$h(-( \tau - t))$$)
- multiply pointwise by $$x$$ (yields $$x(\tau)h(t - \tau)$$)
- integrate over $$\tau$$ to get $$y(t) = \int_{-\infty}^{\infty} x(\tau) h(t - \tau) \, d\tau$$

Example
<to be insert>

### Convolution Evaluation and Properties

#### Convolution Integral
The convolution of an input signal x(t) with an impulse reponse h(t) is

$$y(t) = \int_{-\infty}^{\infty} x(\tau) h_{\tau}(t - \tau) d\tau = (x*h)(t)$$

note: the * notation could be confusing when referring to the textbook as it could have differnet meaning when placing on the left side

**Casual System**

For a causal system $h(t) = 0$ for $t < 0$ and $h(t - \tau) = 0$ for $t > \tau$ by definition, the upper limit of the convolution integral becomes t

$$y(t) = \int_{-\infty}^{t} x(\tau) h_{\tau}(t - \tau) d\tau $$

Now only past and present values of $x(\tau)$ contribtue to $y(t)$

**Causal Input**
For a causal input where $x(t) = 0$ for $t < 0$ , the lower limit of the convolution integral becomes 0 as no input is given before t = 0


$$y(t) = \int_{0}^{\infty} x(\tau) h_{\tau}(t - \tau) d\tau $$

Combine a causal h and a causal x, we get a very simpflied integral of 

$$y(t) = \int_{0}^{t} x(\tau) h_{\tau}(t - \tau) d\tau $$
---
### L3 Summary
For an input $x(t)$, the output of a linear system is given by the superposition integral:  
$$y(t) = \int_{-\infty}^{\infty} x(\tau) h_{\tau}(t) d\tau$$

If the system is also time-invariant, the result is a convolution integral:  
$$y(t) = \int_{-\infty}^{\infty} x(\tau) h(t - \tau) d\tau$$

The response of an LTI system is completely characterized by its impulse response $h(t)$.

Another expression for the superposition integral can be found by substituting $\tau = t - \tau_1$, then $d\tau = -d\tau_1$ and $\tau_1 = t - \tau$:  
$$y(t) = \int_{-\infty}^{\infty} x(\tau) h(t - \tau) d\tau$$  
$$y(t) = \int_{-\infty}^{\infty} x(t - \tau_1) h(t - (t - \tau_1)) d(-\tau_1)$$

---

### System Equation
The system equation relates the outputs of a system to its inputs. Example from last time: the system described by the block diagram:  
$$x \to (+)_{+} \to \text{integral} \to y, \; y \cdot a \to (+)_{-}$$  

This results in:  
$$y' = x - ay$$  
where initial conditions specify a solution.

#### Solutions for the System Equation
The output consists of two components:  
1. **Zero-input response**: The output when $x(t) = 0$.  
2. **Zero-state response**: The output of the system with initial conditions set to zero.

For a linear system $H$, the zero-input response is zero due to homogeneity: if $y = F(ax) = aF(x)$, then $a = 0$ implies $y = 0$.  

---

### Example: Solving for Voltage Across a Capacitor
Find $y(t)$ for an arbitrary input voltage $x(t)$, given $y(0) = Y_0$.  

Circuit:
- $x(t) \to (-+)$, $i(t) \to R \to C \to y(t) \to (-+)x(t)$.  

Using KVL:  
$$x(t) = R i(t) + y(t)$$  
Using $i(t) = C \frac{dy}{dt}$:  
$$x(t) = RC \frac{dy}{dt} + y(t)$$  

Zero-input case:  
$$RC \frac{dy}{dt} + y(t) = 0$$  

Using the first-order ODE solution:  
$$\frac{dy}{dt} + p(t)y = q(t), \; \mu = e^{\int P(t)}$$  
We get:  
$$y(t) = A e^{-t/RC}$$  

For arbitrary input $x(t)$:  
$$RC \left[A'(t)e^{-t/RC} - \frac{1}{RC} A(t)e^{-t/RC}\right] + A(t)e^{-t/RC} = x(t)$$  

Simplifying:  
$$A'(t) = x(t) \cdot \frac{1}{RC} e^{t/RC}$$  
$$A(t) = \int_{0}^{t} x(\tau) \frac{1}{RC} e^{\tau / RC} d\tau + A(0)$$  

Given $y(t) = A(t)e^{-t/RC}$:  
$$y(t) = \left[\int_{0}^{t} x(\tau) \frac{1}{RC} e^{\tau / RC} d\tau + A(0)\right] e^{-t/RC}$$  

At $t = 0$, $y(0) = Y_0 \implies A(0) = Y_0$.  
$$y(t) = \underbrace{\int_{0}^{t} x(\tau) \frac{1}{RC} e^{-(t-\tau)/RC} d\tau}_{\text{Zero-state response}} + \underbrace{Y_0 e^{-t/RC}}_{\text{Zero-input response}}$$  

---

### Impulse Response
The impulse response $h(t)$ is:  
$$h(t) = \frac{1}{RC} e^{-t/RC}$$  

The response of this system to an input $x(t)$ is:  
$$y(t) = \int_{0}^{t} x(\tau) h(t - \tau) d\tau = \int_{0}^{t} x(\tau) \frac{1}{RC} e^{-(t-\tau)/RC} d\tau$$  

This matches the zero-state solution found earlier.

---

### Output of an LTI System
An LTI system $H$ transforms the signal $x(t)$:  
$$x(t) = \int_{-\infty}^{\infty} x(\tau) \delta_{\tau}(t) d\tau$$  

Apply $H$:  
$$y(t) = H\left(\int_{-\infty}^{\infty} x(\tau) \delta_{\tau}(t) d\tau\right)$$  

Resulting in:  
$$y(t) = \int_{-\infty}^{\infty} x(\tau) H(\delta_{\tau}(t))$$  
$$y(t) = \int_{-\infty}^{\infty} x(\tau) h_{\tau}(t) d\tau$$  

For time-invariant systems:  
$$h_{\tau}(t) = h(t - \tau)$$  



### Time-Invariance
For a time-invariant system $H$:  
$$h_{\tau}(t) = h(t - \tau)$$  



### Linearity
A system $S$ is linear if:  
1. **Homogeneity:** If $y = Sx$, then $a y = S(ax)$.  
2. **Superposition:** If $y_1 = Sx_1$ and $y_2 = Sx_2$, then $y_1 + y_2 = S(x_1 + x_2)$.  

Thus:  
$$a y_1 + b y_2 = S(a x_1 + b x_2)$$  

Extended Linearity:
- **Summation:**  
  $$\sum_{n} a_n y_n = S\left(\sum_{n} a_n x_n\right)$$  
- **Integration:**  
  $$\int_{-\infty}^{\infty} a(\tau) y(t - \tau) d\tau = S\left(\int_{-\infty}^{\infty} a(\tau) x(t - \tau) d\tau\right)$$
  
---
### Impulse Response

The impulse response of a linear system, ($h_{\tau}$), is the output of the system at time \(t\) to an impulse at time \(\tau\). For a system (H), this can be written as:  
$$h_{\tau} = H(\delta_{\tau})$$

**Notes:**  
1. A positive ($\tau$) causes a forward shift of the signal and defines the sampling range of ($t - \tau$).  
2. On the left-hand side, \(t\) represents a specific value of time, while on the right-hand side, \(t\) varies over all real numbers (e.g., all time \(t\)). Despite the impulse nature, the specific value of \(t\) on the left depends on this variation.

The equation:  
$$h_{\tau}(t) = H(\delta_{\tau}(t))$$  
can be confusing.  

- At \(\tau = 0\):  
  $$h = h_0 = H(\delta_0)$$  

- Using \(t = 2\) for evaluation:  
  $$h(2) = H(\delta(2))$$  
  implies \(h(2) = H(0)\), which is **incorrect**.

A better notation for the process is:  
$$h(t, \tau) = h(2, 0) - h(t, 0)$$
